
# b)
¬(¬X ∧ Y ∧ Z) ∧ ¬(X ∧ Y ∧ ¬Z) ∧ (X ∧ ¬Y ∧ Z)

# Pojednostavljenje
¬(¬X ∧ Y ∧ Z) ∧ ¬(X ∧ Y ∧ ¬Z) ∧ (X ∧ ¬Y ∧ Z) =\
\= (¬(¬X ∧ Y ∧ Z) ∧ ¬(X ∧ Y ∧ ¬Z)) ∧ (X ∧ ¬Y ∧ Z) =\
\= ¬(¬¬(¬X ∧ Y ∧ Z) ∨ ¬¬(X ∧ Y ∧ ¬Z)) ∧ (X ∧ ¬Y ∧ Z) =\
\= ¬((¬X ∧ Y ∧ Z) ∨ (X ∧ Y ∧ ¬Z)) ∧ (X ∧ ¬Y ∧ Z) =\
\= ¬(Y ∧ ((¬X ∧ Z) ∨ (X ∧ ¬Z))) ∧ (X ∧ ¬Y ∧ Z) =\
\= (¬Y ∨ ¬((¬X ∧ Z) ∨ (X ∧ ¬Z))) ∧ (X ∧ ¬Y ∧ Z) =\
\= (¬Y ∨ (¬(¬X ∧ Z) ∧ ¬(X ∧ ¬Z))) ∧ (X ∧ ¬Y ∧ Z) =\
\= (¬Y ∧ (X ∧ ¬Y ∧ Z)) ∨ (¬(¬X ∧ Z) ∧ ¬(X ∧ ¬Z) ∧ (X ∧ ¬Y ∧ Z)) =\
\= (X ∧ ¬Y ∧ Z) ∨ (¬(¬X ∧ Z) ∧ ¬(X ∧ ¬Z) ∧ (X ∧ ¬Y ∧ Z)) =\
\= (X ∧ ¬Y ∧ Z) ∨ ((¬¬X ∨ ¬Z) ∧ (¬X ∨ ¬¬Z) ∧ (X ∧ ¬Y ∧ Z)) =\
\= (X ∧ ¬Y ∧ Z) ∨ ((X ∨ ¬Z) ∧ (¬X ∨ Z) ∧ (X ∧ ¬Y ∧ Z)) =\
\= (X ∧ ¬Y ∧ Z) ∨ ((X ∧ ¬X ∨ X ∧ Z ∨ ¬Z ∧ ¬X ∨ ¬Z ∧ Z) ∧ (X ∧ ¬Y ∧ Z)) =\
\= (X ∧ ¬Y ∧ Z) ∨ ((X ∧ Z ∨ ¬Z ∧ ¬X) ∧ (X ∧ ¬Y ∧ Z)) =\
\= (X ∧ ¬Y ∧ Z) ∨ ((X ∧ Z ∨ ¬Z ∧ ¬X) ∧ (X ∧ ¬Y ∧ Z)) =\
\= (X ∧ ¬Y ∧ Z) ∨ (X ∧ Z ∧ (X ∧ ¬Y ∧ Z)) ∨ ((¬Z ∧ ¬X) ∧ (X ∧ ¬Y ∧ Z)) =\
\= (X ∧ ¬Y ∧ Z) ∨ (X ∧ ¬Y ∧ Z) ∨ ((¬Z ∧ ¬X) ∧ (X ∧ ¬Y ∧ Z)) =\
\= (X ∧ ¬Y ∧ Z) ∨ (¬Z ∧ ¬X ∧ (X ∧ ¬Y ∧ Z)) =\
\= (X ∧ ¬Y ∧ Z) ∨ (¬Z ∧ ¬X ∧ X ∧ ¬Y ∧ Z) =\
\= (X ∧ ¬Y ∧ Z) ∨ (¬Z ∧ (¬X ∧ X) ∧ ¬Y ∧ Z) =\
\= (X ∧ ¬Y ∧ Z) ∨ (¬Z ∧ 0 ∧ ¬Y ∧ Z) =\
\= X ∧ ¬Y ∧ Z
